celliocb/MaincbIAproof.v
@@ -1,30 +1,28 @@
 Require Import CRIS.
 From CRIS.celliocb Require Import CelliocbHeader CelliocbA MaincbHeader MaincbA MaincbI CtxcbHeader.
 
-Set Implicit Arguments.
 
 Module MaincbIA. Section MaincbIA.
   Import CelliocbA.
-  Context `{!crisG Γ Σ α β τ _S _I}.
-  Context `{_celliocbG: !celliocbG}.
+  Context `{!crisG Γ Σ α β τ _S _I, !concGS}.
+  Context `{_celliocbG: !celliocbGS}.
 
-  Definition Ist: alist key Any.t -> alist key Any.t -> iProp Σ :=
-    λ st_src st_tgt, emp%I.
-
-  Context (sp: sp_type).
-  Context (sp_foo: sp CtxcbHdr.foo = None).
+  Context (sp : specmap).
+  Context (sp_foo: sp !! speckey_fn CtxcbHdr.foo = None).
   
-  Local Definition CelliocbA := (CelliocbA.t).
+  Local Definition CelliocbAMod := (CelliocbA.t).
   Local Definition MaincbA := (MaincbA.t sp).
-  Local Definition IstFull := (IstProd (IstSB MaincbA.(Mod.scopes) Ist) IstEq).
+  Local Definition IstFull := (IstProd (IstSB MaincbA.(Mod.scopes) IstTrue) IstEq).
 
   Lemma simF_main:
-    ISim.sim_fun open MaincbA (MaincbI.t ★ CelliocbA) MaincbA.init_cond IstFull MaincbHdr.main.
+    ISim.sim_fun open MaincbA (MaincbI.t ★ CelliocbAMod) IstFull MaincbHdr.main.
   Proof using sp_foo.
-    init_simF.
+    iStartSim.
+    unfold MaincbA.main, MaincbI.main.
     
     (* Take cell(0) *)
-    steps_l; iDestruct "IST" as "[IST ASM ]"; subst.
+    steps_l.
+    iDestruct "ASM" as "[-> ASM]".
 
     (* Give cell(0) *)
     steps_r. inline_r.
@@ -33,7 +31,7 @@ Module MaincbIA. Section MaincbIA.
     
     (* Inline input_stdin() *)
     steps_r. inline_r.
-    steps_r. 
+    steps_r. unfold MaincbI.input_stdin. 
     
     (* trigger IO together *)
     step. rename ret into i. 
@@ -46,24 +44,19 @@ Module MaincbIA. Section MaincbIA.
 
     (* TGT : inline CellioA.get() *)
     inline_r.
-    steps_r. 
+    steps_r.
+    unfold get. 
     forces_r. 
     iFrame.
 
     steps_r. hss. steps_r.
 
     (* call foo together *)
-    call "IST".
-    {
-      iDestruct "IST" as "[-> ->]".
-      repeat iExists []. iSplit; eauto;
-      repeat unfold_mod; ss;
-      repeat (iSplit; eauto); iPureIntro; prove_scope.
-    }
+    call "IST". iIntros "% % % IST".
 
     (* TGT : handle set(input_db) *)
-    steps_l.
-    steps_r. hss. steps_r.
+    steps_l. steps_r.
+    destruct Any.downcast; steps_l; des_ifs. hss. steps_r.
     
     (* TGT : inline set *)
     inline_r.
@@ -79,6 +72,7 @@ Module MaincbIA. Section MaincbIA.
     steps_r.
 
     (* handle IO together *)
+    unfold MaincbI.input_db.
     step.
     steps_r. hss. 
     steps_r. hss. 
@@ -86,7 +80,7 @@ Module MaincbIA. Section MaincbIA.
     
     (* TGT : inline get *)
     inline_r.
-    steps_r. force_r ret.
+    steps_r. unfold get. force_r ret0.
     
     (* TGT : get cell ret *)
     forces_r. iFrame.
@@ -95,14 +89,16 @@ Module MaincbIA. Section MaincbIA.
     steps_l. 
     
     (* handle IO together *)
-    step. step. iSplit; done.
+    step. steps_l. steps_r. forces_l. iSplit; et. steps_l. step. iFrame; et. 
   (*SLOW*)Qed.
 
   Theorem sim :
-    ISim.t open MaincbA (MaincbI.t ★ CelliocbA) MaincbA.init_cond IstFull.
+    ISim.t open MaincbA (MaincbI.t ★ CelliocbAMod) MaincbA.init_cond IstFull.
   Proof using sp_foo.
     init_sim.
+    - unfold Mod.scopes. hss. unfold MaincbA.scopes. Search submseteq. ⊆+ admit.
     (* - exfalso. revert H0. rewrite /MaincbI.t /CelliocbA. unseal CRIS; ss. *)
+    - iIntros "_". unfold IstFull, IstProd. repeat (iExists ∅). ss. 
     - eapply simF_main; eauto.
   Qed.
 End MaincbIA. End MaincbIA.
