celliocb/MaincbA.v
@@ -1,14 +1,19 @@
 Require Import CRIS.
 Require Import CelliocbA CtxcbHeader CelliocbHeader MaincbHeader.
 
-Set Implicit Arguments.
-
 Module MaincbA. Section MaincbA.
   Import CelliocbA.
-  Context `{!crisG Γ Σ α β τ _S _I}.
-  Context `{_celliocbG: !celliocbG}.
+  Context `{!crisG Γ Σ α β τ _S _I, !concGS}.
+  Context `{_celliocbG: !celliocbGS}.
                 
   Definition scopes := ["Main"].
+
+  Definition main_spec : fspec :=
+    fspec_simple (λ _ : unit, 
+      ((λ arg, (cell 0)), 
+       (λ ret, (True))
+      )
+    )%I.
 
   Definition main: Any.t -> itree crisE Any.t :=
     λ _,
@@ -18,19 +23,18 @@ Module MaincbA. Section MaincbA.
       trigger (@IO _ unit "Print" x);;;
       Ret tt↑.
   
-  Definition fnsems : fnsems_type :=
-    [(MaincbHdr.main, (true, wmask_all, scopes, (None, main)))].
+  Definition fnsems : fnsemmap :=
+    {[MaincbHdr.main := Some ((msk_scp scopes msk_true), (fsp_some main_spec, main))]}.
 
   Program Definition smod : SMod.t := {|
     SMod.scopes := scopes;
     SMod.fnsems := fnsems;
-    SMod.initial_st := [];
+    SMod.initial_st := ∅;
   |}.
-  Solve All Obligations with prove_scope.
-  Next Obligation. prove_nodup. Qed.
+  Solve All Obligations with mod_tac.
 
   Definition init_cond : iProp Σ := cell 0.
 
-  Definition t sp := Seal.sealing CRIS (SMod.to_mod sp smod).
+  Definition t sp := SMod.to_mod sp smod.
 
 End MaincbA. End MaincbA.
